compiler/core/Extraction/ExtrOcamlFloatNatIntZInt.v
@@ -23,57 +23,45 @@ Require Import Float.
 Require Import EquivDec.
 Require Import Extraction.
 
-(** BUG !!! B755_zero false = +0 ; B755_zero true = -0 *)
-(** BUG !!! SAME FOR INFINITY *)
-Extract Inductive Fappli_IEEE.binary_float => float [
-  "(fun s -> if s then (-0.) else (0.))"
-  "(fun s -> if s then neg_infinity else infinity)"
-  "nan"
-  "(fun (s, m, e) -> if s then -. (ldexp (float_of_int m) e) else (ldexp (float_of_int m) e))"
-].
-Extract Inlined Constant nan => "nan".
-Extract Inlined Constant zero => "0.".
-Extract Inlined Constant neg_zero => "(-0.)".
-Extract Inlined Constant one => "1.".
-Extract Inlined Constant neg_one => "(-1.)".
-Extract Inlined Constant infinity => "infinity".
-Extract Inlined Constant neg_infinity => "neg_infinity".
-Extract Inlined Constant max_value => "max_float".
-Extract Inlined Constant min_value => "(Int64.float_of_bits Int64.one)". (** XXX Why not min_float in OCaml? *)
+(* PrimFloat.float extraction via ExtrOCamlFloats depends on the kernel float Float64 library.
+   This is annoying for building, and also causes problems because the type t is opaque
+   and there is no non-magic way to get a float out of it
+ *)
 
-Extract Inlined Constant float_floor => "(fun x -> floor x)".
-Extract Inlined Constant float_absolute => "(fun x -> abs_float x)".
-Extract Inlined Constant float_neg => "(fun x -> ~-. x)".
+Extract Inlined Constant PrimFloat.float => "float".
+Extract Inlined Constant float => "float".
+
+Extract Inlined Constant float_nan => "Float.nan".
+Extract Inlined Constant float_zero => "0.".
+Extract Inlined Constant float_neg_zero => "(-0.)".
+Extract Inlined Constant float_one => "1.".
+Extract Inlined Constant float_neg_one => "(-1.)".
+Extract Inlined Constant float_infinity => "Float.infinity".
+Extract Inlined Constant float_neg_infinity => "Float.neg_infinity".
+
+(*
+Extract Inductive FloatClass.float_class =>
+  "Float64.float_class"
+  [ "PNormal" "NNormal" "PSubn" "NSubn" "PZero" "NZero" "PInf" "NInf" "NaN" ].
+Extract Inductive PrimFloat.float_comparison =>
+  "Float64.float_comparison"
+    [ "FEq" "FLt" "FGt" "FNotComparable" ].
+
+*)
+Extract Inlined Constant float_max_value => "Float.max_float".
+Extract Inlined Constant float_min_value => "Float.min_value".
+
+Extract Inlined Constant float_from_string => "(fun x -> float_of_string (Util.string_of_char_list x))".
+Extract Inlined Constant float_to_string => "(fun x -> Util.char_list_of_string (Util.qcert_string_of_float x))".
+
+Extract Inlined Constant float_neg => "(fun x -> Float.neg x)".
+
+Extract Inlined Constant float_floor => "(fun x -> Float.floor x)".
+Extract Inlined Constant float_absolute => "(fun x -> Float.abs x)".
+
+Extract Inlined Constant float_sign => "(fun x -> Util.float_sign x)".
 
 (** Defines additional operations on FLOATs *)
-(** Unary operations *)
-
-Extract Inlined Constant float_sqrt => "(fun x -> sqrt x)".
-Extract Inlined Constant float_exp => "(fun x -> exp x)".
-Extract Inlined Constant float_log => "(fun x -> log x)".
-Extract Inlined Constant float_log10 => "(fun x -> log10 x)".
-Extract Inlined Constant float_ceil => "(fun x -> ceil x)".
-
-Extract Inlined Constant float_eq => "(fun x y -> x = y)".
-
-Conjecture float_eq_correct :
-  forall f1 f2, (float_eq f1 f2 = true <-> f1 = f2).
-Lemma float_eq_dec : EqDec float eq.
-Proof.
-  unfold EqDec.
-  intros x y.
-  case_eq (float_eq x y); intros eqq.
-  + left.
-    f_equal.
-    apply float_eq_correct in eqq.
-    trivial.
-  + right; intros eqq2.
-    red in eqq2.
-    apply float_eq_correct in eqq2.
-    congruence.
-Defined.
-  
-Extract Constant float_eq_dec => "(fun n1 n2 -> 0 = compare n1 n2)".
 
 (** Binary operations *)
 Extract Inlined Constant float_add => "(fun x y -> x +. y)".
@@ -81,20 +69,30 @@ Extract Inlined Constant float_sub => "(fun x y -> x -. y)".
 Extract Inlined Constant float_mult => "(fun x y -> x *. y)".
 Extract Inlined Constant float_div => "(fun x y -> x /. y)".
 
+(** Unary operations *)
+Extract Inlined Constant float_sqrt => "(fun x -> Float.sqrt x)".
+Extract Inlined Constant float_exp => "(fun x -> Float.exp x)".
+Extract Inlined Constant float_log => "(fun x -> Float.log x)".
+Extract Inlined Constant float_log10 => "(fun x -> Float.log10 x)".
+Extract Inlined Constant float_ceil => "(fun x -> Float.ceil x)".
+
+Extract Constant float_eq => "(fun n1 n2 -> n1 = n2)".
+(* Extract Constant float_eq_dec => "(fun n1 n2 -> n1 = n2)". *)
+
+
 Extract Inlined Constant float_pow => "(fun x y -> x ** y)".
 Extract Inlined Constant float_min => "(fun x y -> min x y)".
 Extract Inlined Constant float_max => "(fun x y -> max x y)".
 Extract Inlined Constant float_ne => "(fun x y -> x <> y)".
+
 Extract Inlined Constant float_lt => "(fun x y -> x < y)".
-Extract Inlined Constant float_le => "(fun x y -> x <= y)".
-Extract Inlined Constant float_gt => "(fun x y -> x > y)".
-Extract Inlined Constant float_ge => "(fun x y -> x >= y)".
+Extract Inlined Constant float_le  => "(fun x y -> x <= y)".
+Extract Inlined Constant float_gt  => "(fun x y -> x > y)".
+Extract Inlined Constant float_ge  => "(fun x y -> x >= y)".
 
 Require Import ZArith.
 Extract Inlined Constant float_of_int => "(fun x -> float_of_int x)".
 
 Extract Inlined Constant float_truncate => "(fun x -> truncate x)".
 
-Extract Inlined Constant from_string => "(fun x -> float_of_string (Util.string_of_char_list x))".
-Extract Inlined Constant to_string => "(fun x -> Util.char_list_of_string (Util.qcert_string_of_float x))".
-
+Extract Inlined Constant JsNumber.to_string => "(fun x -> Util.char_list_of_string (Util.qcert_string_of_float x))".
