compiler/core/NNRC/Optim/NNRCOptimizer.v
@@ -17,6 +17,7 @@
 Require Import String.
 Require Import List.
 Require Import ListSet.
+Require Import BinInt.
 Require Import Arith.
 Require Import Equivalence.
 Require Import Morphisms.
